examples/bst.v
@@ -1,0 +1,268 @@
+From Coq Require Import ssreflect ssrbool ssrfun.
+From mathcomp Require Import eqtype ssrnat seq path.
+From fcsl Require Import axioms pred ordtype.
+From fcsl Require Import pcm unionmap heap autopcm automap.
+From HTT Require Import model heapauto.
+From HTT Require Import bintree.
+Set Implicit Arguments.
+Unset Strict Implicit.
+Unset Printing Implicit Defensive.
+Obligation Tactic := auto.
+
+Section BST.
+Context {T : ordType}.
+
+(* Helper lemmas *)
+
+Lemma iffPb (b1 b2 : bool) : reflect (b1 <-> b2) (b1 == b2).
+Proof.
+case: eqP=>[->|N]; constructor=>//.
+case: b1 b2 N; case=>//= _.
+- by case=>/(_ erefl).
+by case=>_ /(_ erefl).
+Qed.
+
+Lemma iffE (b1 b2 : bool) : b1 = b2 <-> (b1 <-> b2).
+Proof. by split=>[->|] //; move/iffPb/eqP. Qed.
+Lemma ord_neq (x y : T) : ord x y -> x != y.
+Proof.
+move=>H; apply/negP=>/eqP E.
+by rewrite E irr in H.
+Qed.
+
+Lemma all_notin {A : eqType} (p : pred A) xs y :
+  all p xs -> ~~ p y -> y \notin xs.
+Proof. by move/allP=>Ha; apply/contra/Ha. Qed.
+
+Lemma sorted_rconsE (xs : seq T) x :
+  sorted ord (rcons xs x) = all (ord^~ x) xs && sorted ord xs.
+Proof.
+rewrite -(revK (rcons _ _)) rev_rcons rev_sorted /= path_sortedE; last first.
+- by move=>a b c Hab /trans; apply.
+by rewrite all_rev rev_sorted.
+Qed.
+
+Lemma sorted_cat_cons_cat (l r : seq T) x :
+  sorted ord (l ++ x :: r) = sorted ord (l ++ [::x]) && sorted ord (x::r).
+Proof.
+apply/iffE; split.
+- by move/[dup]/cat_sorted2=>->; rewrite -cat1s catA =>/cat_sorted2 ->.
+case/andP=>/= + H; rewrite cats1.
+case: l=>//=a l; rewrite rcons_path=>/andP [H1 H2].
+by rewrite cat_path /= H1 H2.
+Qed.
+
+(* bst operations *)
+
+Fixpoint insert x (t : tree T) : tree T :=
+  if t is Node l a r
+    then
+      if x == a then Node l a r
+        else if ord x a then Node (insert x l) a r
+                        else Node l a (insert x r)
+  else Node leaf x leaf.
+
+Fixpoint search (t : tree T) x : bool :=
+  if t is Node l a r
+    then
+      if x == a then true
+        else if ord x a then search l x
+                        else search r x
+  else false.
+
+(* invariant *)
+
+Fixpoint bst (t : tree T) : bool :=
+  if t is Node l a r
+    then [&& all (ord^~ a) (inorder l), all (ord a) (inorder r), bst l & bst r]
+    else true.
+
+Lemma bst_to_sorted (t : tree T) :
+  bst t <-> sorted ord (inorder t).
+Proof.
+elim: t=>//=l IHl a r IHr.
+rewrite sorted_cat_cons_cat /= cats1 (sorted_rconsE) (path_sortedE (@trans T)) -andbA.
+split; case/and4P.
+- by move=>->->/IHl->/IHr->.
+by move=>->/IHl->->/IHr->.
+Qed.
+
+Lemma inorder_insert x (t : tree T) :
+  bst t ->
+  perm_eq (inorder (insert x t))
+          (if x \in inorder t then inorder t else x :: inorder t).
+Proof.
+elim: t=>//=l IHl a r IHr /and4P [Hal Har /IHl Hl /IHr Hr] {IHl IHr}.
+rewrite mem_cat inE; case: (ifP [|| _, _ | _]).
+- case/or3P=>H.
+  - rewrite H in Hl.
+    move/allP: Hal=>/(_ x H) /[dup] Hxa /ord_neq/negbTE ->; rewrite Hxa /=.
+    by apply/permEl/perm_catr.
+  - by rewrite H.
+  rewrite H in Hr.
+  move/allP: Har=>/(_ x H) /[dup] /nsym/negP/negbTE ->.
+  move/ord_neq; rewrite eq_sym =>/negbTE -> /=.
+  by apply/permEl/perm_catl; rewrite perm_cons.
+move/negbT; rewrite !negb_or; case/and3P=>/negbTE Hxl /negbTE Hx /negbTE Hxr.
+rewrite {}Hxl in Hl; rewrite {}Hxr in Hr; case: (ordP x a)=>/= H.
+- by rewrite -cat_cons; apply/permEl/perm_catr.
+- by rewrite H in Hx.
+rewrite -(cat1s x) -(cat1s a) -(cat1s a (inorder r)).
+rewrite perm_sym perm_catC -!catA catA perm_sym catA.
+apply/permEl/perm_catl; apply: (perm_trans Hr).
+by rewrite cats1 -perm_rcons.
+Qed.
+
+Lemma bst_insert x (t : tree T) : bst t -> bst (insert x t).
+Proof.
+elim: t=>//=l IHl a r IHr /and4P [Hal Har Hl Hr].
+case: ifP; first by move=>_ /=; rewrite Hal Har Hl Hr.
+move=>Hx; case: ifP=>Ho /=.
+- rewrite Har (IHl Hl) Hr /= andbT (perm_all _ (@inorder_insert x _ Hl)).
+  by case: ifP=>//= _; rewrite Ho.
+rewrite Hal Hl (IHr Hr) /= andbT (perm_all _ (@inorder_insert x _ Hr)).
+case: ifP=>//= _; rewrite Har andbT.
+by case: ordP=>//; [rewrite Ho| rewrite Hx].
+Qed.
+
+Lemma insert_insert x1 x2 (t : tree T) :
+  bst t ->
+  perm_eq (inorder (insert x1 (insert x2 t)))
+          (inorder (insert x2 (insert x1 t))).
+Proof.
+move=>H.
+have H1: (bst (insert x1 t)) by apply: bst_insert.
+have H2: (bst (insert x2 t)) by apply: bst_insert.
+apply: (perm_trans (inorder_insert x1 H2)); rewrite perm_sym.
+apply: (perm_trans (inorder_insert x2 H1)).
+rewrite (perm_mem (inorder_insert x1 H) x2) (perm_mem (inorder_insert x2 H) x1).
+case: (ifP (x1 \in _))=>Hx1.
+- case: (ifP (x2 \in _))=>Hx2.
+  - apply: (perm_trans (inorder_insert x1 H)); rewrite Hx1 perm_sym.
+    by apply: (perm_trans (inorder_insert x2 H)); rewrite Hx2.
+  - rewrite inE Hx1 orbT perm_sym.
+    apply: (perm_trans (inorder_insert x2 H)); rewrite Hx2 perm_cons perm_sym.
+    by apply: (perm_trans (inorder_insert x1 H)); rewrite Hx1.
+rewrite inE; case: ifP.
+- case/orP.
+  - by move/eqP=>->; rewrite Hx1 inE eq_refl /=.
+  move=>Hx2; rewrite Hx2 Hx1.
+  apply: (perm_trans (inorder_insert x1 H)); rewrite Hx1 perm_cons perm_sym.
+  by apply: (perm_trans (inorder_insert x2 H)); rewrite Hx2.
+move/negbT; rewrite negb_or; case/andP=>/negbTE HE /negbTE Hx2.
+rewrite Hx2 inE Hx1 orbF eq_sym HE.
+move: (inorder_insert x1 H); rewrite -(perm_cons x2) Hx1=>H'; apply: (perm_trans H').
+rewrite -cat1s -(cat1s x1) perm_catCA /= perm_cons perm_sym.
+by apply: (perm_trans (inorder_insert x2 H)); rewrite Hx2.
+Qed.
+
+Lemma inorder_search (t : tree T) :
+  bst t ->
+  search t =i inorder t.
+Proof.
+move=>+ x; elim: t=>//=l IHl a r IHr /and4P [Hal Har /IHl Hl /IHr Hr] {IHl IHr}.
+rewrite -topredE /= in Hl; rewrite -topredE /= in Hr.
+rewrite -topredE /= mem_cat inE.
+case: ifP=>_ /=; first by rewrite orbT.
+case: ifP=>Hx.
+- rewrite Hl.
+  suff: x \notin inorder r by move/negbTE=>->/=; rewrite orbF.
+  by apply: (all_notin Har); apply/negP/nsym.
+rewrite Hr.
+suff: x \notin inorder l by move/negbTE=>->.
+by apply: (all_notin Hal)=>/=; rewrite Hx.
+Qed.
+
+(* Procedures *)
+
+Opaque mknode.
+
+Definition inserttreeT x : Type :=
+  forall p, {t : tree T}, STsep (treep p t, [vfun p' => treep p' (insert x t)]).
+
+Program Definition inserttree x : inserttreeT x :=
+  Fix (fun (go : inserttreeT x) p =>
+       Do (if p == null
+             then n <-- mknode x;
+                  ret n
+             else a <-- !(p.+ 1);
+                  if x == a then ret p
+                    else if ord x a then l <-- !p;
+                                         l' <-- go l;
+                                         p ::= l';;
+                                         ret p
+                                    else r <-- !(p.+ 2);
+                                         r' <-- go r;
+                                         p.+ 2 ::= r';;
+                                         ret p)).
+Next Obligation.
+move=>x go p [t][] i /= H.
+case: eqP H=>[{p}->|/eqP E] H.
+- apply: vrfV=>V; case: (treep_null V H)=>{t H}->{i V}->.
+  by apply: [stepE]=>//=; case=>//= n m H; step.
+case: (treep_cont E H)=>l[z][r][pl][pr][_][{t H}->{i}->][hl][hr][-> Hl Hr].
+step; case: eqP.
+- move=>_; step=>_.
+  by exists pl, pr, (hl \+ hr); split=>//; exists hl, hr.
+move=>Exz; case: ifP=>Ho; step.
+- apply: [stepX l]@hl=>//= p' h' H'.
+  do 2![step]=>{pl Hl} _.
+  by exists p', pr, (h' \+ hr); split=>//; exists h', hr.
+apply: [stepX r]@hr=>//= p' h' H'.
+do 2![step]=>{pr Hr} _.
+by exists pl, p', (hl \+ h'); split=>//; exists hl, h'.
+Qed.
+
+Definition searchtreeT x : Type :=
+  forall p, {t : tree T}, STsep (treep p t, [vfun b h => treep p t h /\ b == search t x]).
+
+Program Definition searchtree x : searchtreeT x :=
+  Fix (fun (go : searchtreeT x) p =>
+       Do (if p == null
+             then ret false
+             else a <-- !(p.+ 1);
+                  if x == a then ret true
+                    else if ord x a then l <-- !p;
+                                         go l
+                                    else r <-- !(p.+ 2);
+                                         go r)).
+Next Obligation.
+move=>x go p [t][] i /= H.
+case: eqP H=>[{p}->|/eqP E] H.
+- apply: vrfV=>V; case: (treep_null V H)=>{t H}->{i V}->.
+  by step.
+case: (treep_cont E H)=>l[z][r][pl][pr][_][{t H}->{i}->][hl][hr][-> Hl Hr].
+step; case: eqP.
+- move=>_; step=>_; split=>//.
+  by exists pl, pr, (hl \+ hr); split=>//; exists hl, hr.
+move=>Exz; case: ifP=>Ho; step.
+- apply: [gX l]@hl=>//= b h' [H' E'] _; split=>{b E' hl Hl}//.
+  by exists pl, pr, (h' \+ hr); split=>//; exists h', hr.
+apply: [gX r]@hr=>//= b h' [H' E'] _; split=>{b E' hr Hr}//.
+by exists pl, pr, (hl \+ h'); split=>//; exists hl, h'.
+Qed.
+
+Program Definition test p x1 x2 :
+  {t : tree T}, STsep (fun h => treep p t h /\ bst t,
+                      [vfun (pb : ptr * bool) h =>
+                       let t' := insert x2 (insert x1 t) in
+                       [/\ treep pb.1 t' h, bst t' & pb.2]]) :=
+  Do (p1 <-- inserttree x1 p;
+      p2 <-- inserttree x2 p1;
+      r <-- searchtree x1 p2;
+      ret (p2, r)).
+Next Obligation.
+move=>p x1 x2 [t][] i /= [Ht Hi].
+apply: [stepE t]=>//=; case=>//= p1 h1 H1.
+apply: [stepE (insert x1 t)]=>//=; case=>//= p2 h2 H2.
+apply: [stepE (insert x2 (insert x1 t))]=>//=; case=>//= b h3 [H3 Hb].
+step=>_.
+have Hr2: bst (insert x2 t) by apply: bst_insert.
+have Hr21: bst (insert x2 (insert x1 t)) by do 2![apply: bst_insert].
+split=>//; rewrite (eqP Hb).
+move: (inorder_search Hr21 x1); rewrite -topredE /= =>->.
+rewrite (perm_mem (insert_insert _ _ Hi)) (perm_mem (inorder_insert x1 Hr2) x1).
+by case: ifP=>// _; rewrite inE eq_refl.
+Qed.
+
+End BST.
